src/ProbabilisticProgramming/WhileAndUntil.dfy
@@ -9,46 +9,46 @@ include "Independence.dfy"
 include "RandomNumberGenerator.dfy"
 
 module WhileAndUntil {
-  import opened Monad
-  import opened Quantifier
-  import opened Independence
-  import opened RandomNumberGenerator
+  import Monad
+  import Quantifier
+  import Independence
+  import RandomNumberGenerator
 
   /************
    Definitions  
   ************/
 
   // Definition 37
-  function ProbWhileCut<A>(c: A -> bool, b: A -> Hurd<A>, n: nat, a: A): Hurd<A> {
+  function ProbWhileCut<A>(c: A -> bool, b: A -> Monad.Hurd<A>, n: nat, a: A): Monad.Hurd<A> {
     if n == 0 then
-      Return(a)
+      Monad.Return(a)
     else (
            if c(a) then
-             Bind(b(a), (a': A) => ProbWhileCut(c, b, n-1, a'))
+             Monad.Bind(b(a), (a': A) => ProbWhileCut(c, b, n-1, a'))
            else
-             Return(a)
+             Monad.Return(a)
          )
   }
 
   // Definition 39 / True iff mu(iset s | ProbWhile(c, b, a)(s) terminates) == 1
-  ghost predicate ProbWhileTerminates<A(!new)>(b: A -> Hurd<A>, c: A -> bool) {
+  ghost predicate ProbWhileTerminates<A(!new)>(b: A -> Monad.Hurd<A>, c: A -> bool) {
     var P := (a: A) => 
-      (s: RNG) => exists n :: !c(ProbWhileCut(c, b, n, a)(s).0);
-    forall a :: ForAllStar(P(a))
+      (s: RandomNumberGenerator.RNG) => exists n :: !c(ProbWhileCut(c, b, n, a)(s).0);
+    forall a :: Quantifier.ForAllStar(P(a))
   }
 
   // Theorem 38
-  function ProbWhile<A>(c: A -> bool, b: A -> Hurd<A>, a: A): (f: Hurd<A>)
+  function ProbWhile<A>(c: A -> bool, b: A -> Monad.Hurd<A>, a: A): (f: Monad.Hurd<A>)
     requires ProbWhileTerminates(b, c)
   {
     assume {:axiom} false;
     if c(a) then
-      Bind(b(a), (a': A) => ProbWhile(c, b, a'))
+      Monad.Bind(b(a), (a': A) => ProbWhile(c, b, a'))
     else
-      Return(a)
+      Monad.Return(a)
   }
 
-  method ProbWhileImperative<A>(c: A -> bool, b: A -> Hurd<A>, a: A, s: RNG) returns (t: (A, RNG)) 
+  method ProbWhileImperative<A>(c: A -> bool, b: A -> Monad.Hurd<A>, a: A, s: RandomNumberGenerator.RNG) returns (t: (A, RandomNumberGenerator.RNG)) 
     requires ProbWhileTerminates(b, c)
     ensures ProbWhile(c, b, a)(s) == t
     decreases *
@@ -61,7 +61,7 @@ module WhileAndUntil {
     return (a, s);
   }
 
-  method ProbWhileImperativeAlternative<A>(c: A -> bool, b: A -> Hurd<A>, a: A, s: RNG) returns (t: (A, RNG)) 
+  method ProbWhileImperativeAlternative<A>(c: A -> bool, b: A -> Monad.Hurd<A>, a: A, s: RandomNumberGenerator.RNG) returns (t: (A, RandomNumberGenerator.RNG)) 
     requires ProbWhileTerminates(b, c)
     ensures ProbWhile(c, b, a)(s) == t
     decreases *
@@ -77,14 +77,14 @@ module WhileAndUntil {
     }
   }
 
-  ghost predicate ProbUntilTerminates<A(!new)>(b: Hurd<A>, c: A -> bool) {
+  ghost predicate ProbUntilTerminates<A(!new)>(b: Monad.Hurd<A>, c: A -> bool) {
     var c' := (a: A) => !c(a);
     var b' := (a: A) => b;
     ProbWhileTerminates(b', c')
   }
 
   // Definition 44
-  function ProbUntil<A>(b: Hurd<A>, c: A -> bool): (f: Hurd<A>)
+  function ProbUntil<A>(b: Monad.Hurd<A>, c: A -> bool): (f: Monad.Hurd<A>)
     requires ProbUntilTerminates(b, c)
     ensures 
       var c' := (a: A) => !c(a);
@@ -93,10 +93,10 @@ module WhileAndUntil {
   {
     var c' := (a: A) => !c(a);
     var b' := (a: A) => b;
-    Bind(b, (a: A) => ProbWhile(c', b', a))
+    Monad.Bind(b, (a: A) => ProbWhile(c', b', a))
   }
 
-  method ProbUntilImperative<A>(b: Hurd<A>, c: A -> bool, s: RNG) returns (t: (A, RNG))
+  method ProbUntilImperative<A>(b: Monad.Hurd<A>, c: A -> bool, s: RandomNumberGenerator.RNG) returns (t: (A, RandomNumberGenerator.RNG))
     requires ProbUntilTerminates(b, c)
     ensures t == ProbUntil(b, c)(s)
     decreases *
@@ -106,24 +106,24 @@ module WhileAndUntil {
     t := ProbWhileImperative(c', b', b(s).0, b(s).1);
   }
 
-  function Helper<A(!new)>(b: A -> Hurd<A>, c: A -> bool, a: A): (RNG -> bool) {
-    (s: RNG) =>
+  function Helper<A(!new)>(b: A -> Monad.Hurd<A>, c: A -> bool, a: A): (RandomNumberGenerator.RNG -> bool) {
+    (s: RandomNumberGenerator.RNG) =>
       !c(b(a)(s).0)
   }
 
-  function Helper2<A(!new)>(b: Hurd<A>, c: A -> bool): (RNG -> bool) {
-    (s: RNG) =>
+  function Helper2<A(!new)>(b: Monad.Hurd<A>, c: A -> bool): (RandomNumberGenerator.RNG -> bool) {
+    (s: RandomNumberGenerator.RNG) =>
       c(b(s).0)
   }
 
-  function Helper3<A>(b: Hurd<A>, c: A -> bool): (RNG -> bool)
+  function Helper3<A>(b: Monad.Hurd<A>, c: A -> bool): (RandomNumberGenerator.RNG -> bool)
     requires ProbUntilTerminates(b, c)
   {
-    (s: RNG) =>
+    (s: RandomNumberGenerator.RNG) =>
       c(ProbUntil(b, c)(s).0)
   }
 
-  ghost function ConstructEvents<A>(b: Hurd<A>, c: A -> bool, d: A -> bool): (x: (iset<RNG>, iset<RNG>, iset<RNG>))
+  ghost function ConstructEvents<A>(b: Monad.Hurd<A>, c: A -> bool, d: A -> bool): (x: (iset<RandomNumberGenerator.RNG>, iset<RandomNumberGenerator.RNG>, iset<RandomNumberGenerator.RNG>))
     requires ProbUntilTerminates(b, c)
   {
     (iset s | d(ProbUntil(b, c)(s).0), iset s | d(b(s).0) && c(b(s).0), iset s | c(b(s).0))
@@ -133,20 +133,20 @@ module WhileAndUntil {
    Lemmas  
   *******/
 
-  lemma EnsureProbUntilTerminates<A(!new)>(b: Hurd<A>, c: A -> bool)
-    requires IsIndepFn(b)
-    requires ExistsStar((s: RNG) => c(b(s).0))
+  lemma EnsureProbUntilTerminates<A(!new)>(b: Monad.Hurd<A>, c: A -> bool)
+    requires Independence.IsIndepFn(b)
+    requires Quantifier.ExistsStar((s: RandomNumberGenerator.RNG) => c(b(s).0))
     ensures ProbUntilTerminates(b, c)
   {
     var c' := (a: A) => !c(a);
     var b' := (a: A) => b;
-    var p := (s: RNG) => c(b(s).0);
+    var p := (s: RandomNumberGenerator.RNG) => c(b(s).0);
     assert ProbUntilTerminates(b, c) by {
-      forall a: A ensures IsIndepFn(b'(a)) {
+      forall a: A ensures Independence.IsIndepFn(b'(a)) {
         assert b'(a) == b;
       }
-      forall a: A ensures ExistsStar(Helper(b', c', a)) {
-        assert ExistsStar(p);
+      forall a: A ensures Quantifier.ExistsStar(Helper(b', c', a)) {
+        assert Quantifier.ExistsStar(p);
         assert (iset s | p(s)) == (iset s | Helper(b', c', a)(s));
       }
       assert ProbWhileTerminates(b', c') by {
@@ -156,39 +156,39 @@ module WhileAndUntil {
   }
 
   // (Equation 3.30) / Sufficient conditions for while-loop termination
-  lemma {:axiom} EnsureProbWhileTerminates<A(!new)>(b: A -> Hurd<A>, c: A -> bool)
-    requires forall a :: IsIndepFn(b(a))
-    requires forall a :: ExistsStar(Helper(b, c, a))
+  lemma {:axiom} EnsureProbWhileTerminates<A(!new)>(b: A -> Monad.Hurd<A>, c: A -> bool)
+    requires forall a :: Independence.IsIndepFn(b(a))
+    requires forall a :: Quantifier.ExistsStar(Helper(b, c, a))
     ensures ProbWhileTerminates(b, c)
 
   // Theorem 45 (wrong!) / PROB_BERN_UNTIL (correct!)
-  lemma {:axiom} ProbUntilProbabilityFraction<A>(b: Hurd<A>, c: A -> bool, d: A -> bool)
-    requires IsIndepFn(b)
-    requires ExistsStar(Helper2(b, c))
+  lemma {:axiom} ProbUntilProbabilityFraction<A>(b: Monad.Hurd<A>, c: A -> bool, d: A -> bool)
+    requires Independence.IsIndepFn(b)
+    requires Quantifier.ExistsStar(Helper2(b, c))
     ensures ProbUntilTerminates(b, c)
     ensures
       var x := ConstructEvents(b, c, d);
-      && x.0 in event_space
-      && x.1 in event_space
-      && x.2 in event_space
-      && mu(x.2) != 0.0
-      && mu(x.0) == mu(x.1) / mu(x.2)
+      && x.0 in RandomNumberGenerator.event_space
+      && x.1 in RandomNumberGenerator.event_space
+      && x.2 in RandomNumberGenerator.event_space
+      && RandomNumberGenerator.mu(x.2) != 0.0
+      && RandomNumberGenerator.mu(x.0) == RandomNumberGenerator.mu(x.1) / RandomNumberGenerator.mu(x.2)
 
   // Equation (3.39)
-  lemma {:axiom} ProbUntilAsBind<A(!new)>(b: Hurd<A>, c: A -> bool, s: RNG)
-    requires IsIndepFn(b)
-    requires ExistsStar(Helper2(b, c))
+  lemma {:axiom} ProbUntilAsBind<A(!new)>(b: Monad.Hurd<A>, c: A -> bool, s: RandomNumberGenerator.RNG)
+    requires Independence.IsIndepFn(b)
+    requires Quantifier.ExistsStar(Helper2(b, c))
     ensures ProbUntilTerminates(b, c)
-    ensures ProbUntil(b, c) == Bind(b, (x: A) => if c(x) then Return(x) else ProbUntil(b, c))
+    ensures ProbUntil(b, c) == Monad.Bind(b, (x: A) => if c(x) then Monad.Return(x) else ProbUntil(b, c))
 
   // Equation (3.40)
-  lemma EnsureProbUntilTerminatesAndForAll<A(!new)>(b: Hurd<A>, c: A -> bool)
-    requires IsIndepFn(b)
-    requires ExistsStar(Helper2(b, c))
+  lemma EnsureProbUntilTerminatesAndForAll<A(!new)>(b: Monad.Hurd<A>, c: A -> bool)
+    requires Independence.IsIndepFn(b)
+    requires Quantifier.ExistsStar(Helper2(b, c))
     ensures ProbUntilTerminates(b, c)
-    ensures ForAllStar(Helper3(b, c))
+    ensures Quantifier.ForAllStar(Helper3(b, c))
   {
     EnsureProbUntilTerminates(b, c);
-    assume {:axiom} ForAllStar(Helper3(b, c));
+    assume {:axiom} Quantifier.ForAllStar(Helper3(b, c));
   }
 }
