src/Distributions/BernoulliRational/Implementation.dfy
@@ -8,9 +8,9 @@ include "Model.dfy"
 
 module BernoulliRationalImplementation {
   import BernoulliRationalModel
-  import opened BernoulliRationalInterface
+  import BernoulliRationalInterface
 
-  trait {:termination false} TBernoulliRational extends IBernoulliRational {
+  trait {:termination false} TBernoulliRational extends BernoulliRationalInterface.IBernoulliRational {
 
    method BernoulliRational(m: nat, n: nat) returns (c: bool)
       modifies this
